feat(*) fine-tuning

HOTG/Orders/HOTG_Additively_Divides.thy
@@ -1,25 +1,29 @@
-theory HOTG_Additive_Order
-  imports HOTG_Addition
+\<^marker>\<open>creator "Niklas Krofta"\<close>
+theory HOTG_Additively_Divides
+  imports
+    HOTG_Addition
+    Transport.Functions_Base
 begin
 
-definition additively_divides :: "set \<Rightarrow> set \<Rightarrow> bool" where
-"additively_divides x y \<longleftrightarrow> (\<exists>d. x + d = y)"
+unbundle no_HOL_groups_syntax
 
-bundle hotg_additive_order_syntax begin notation additively_divides (infix "\<unlhd>" 50) end
-bundle no_hotg_additive_order_syntax begin no_notation additively_divides (infix "\<unlhd>" 50) end
-unbundle hotg_additive_order_syntax
+definition "additively_divides x y \<equiv> has_inverse ((+) x) y"
 
-lemma additively_dividesI[intro]:
+bundle hotg_additively_divides_syntax begin notation additively_divides (infix "\<unlhd>" 50) end
+bundle no_hotg_additively_divides_syntax begin no_notation additively_divides (infix "\<unlhd>" 50) end
+unbundle hotg_additively_divides_syntax
+
+lemma additively_dividesI [intro]:
   assumes "x + d = y"
   shows "x \<unlhd> y"
   unfolding additively_divides_def using assms by auto
 
-lemma additively_dividesE[elim]:
+lemma additively_dividesE [elim]:
   assumes "x \<unlhd> y"
   obtains d where "x + d = y"
   using assms unfolding additively_divides_def by auto
 
-lemma subset_if_additively_divides: "x \<unlhd> y \<Longrightarrow> x \<subseteq> y" 
+lemma subset_if_additively_divides: "x \<unlhd> y \<Longrightarrow> x \<subseteq> y"
   using add_eq_bin_union_lift by force
 
 lemma le_if_additively_divides: "x \<unlhd> y \<Longrightarrow> x \<le> y"
@@ -31,7 +35,7 @@ lemma reflexive_additively_divides: "reflexive (\<unlhd>)"
 lemma antisymmetric_additively_divides: "antisymmetric (\<unlhd>)"
   using subset_if_additively_divides by auto
 
-lemma additively_divides_trans[trans]: "x \<unlhd> y \<Longrightarrow> y \<unlhd> z \<Longrightarrow> x \<unlhd> z"
+lemma additively_divides_trans [trans]: "x \<unlhd> y \<Longrightarrow> y \<unlhd> z \<Longrightarrow> x \<unlhd> z"
   using add_assoc by force
 
 corollary transitive_additively_divides: "transitive (\<unlhd>)"
@@ -40,41 +44,36 @@ corollary transitive_additively_divides: "transitive (\<unlhd>)"
 corollary preorder_additively_divides: "preorder (\<unlhd>)"
   using reflexive_additively_divides transitive_additively_divides by blast
 
-corollary additively_divides_partial_order: "partial_order (\<unlhd>)"
+corollary partial_order_additively_divides: "partial_order (\<unlhd>)"
   using preorder_additively_divides antisymmetric_additively_divides by auto
 
-lemma additively_divides_if_sums_equal:
+lemma additively_divides_or_additively_divides_if_add_eq_add:
   assumes "a + b = c + d"
   shows "a \<unlhd> c \<or> c \<unlhd> a"
 proof (rule ccontr)
-  assume ac_incomparable: "\<not> (a \<unlhd> c \<or> c \<unlhd> a)"
+  assume ac_incomparable: "\<not>(a \<unlhd> c \<or> c \<unlhd> a)"
   have "\<forall>z. a + x \<noteq> c + z" for x
   proof (induction x rule: mem_induction)
-    case (mem x)
-    show ?case
+    case (mem x) show ?case
     proof (cases "x = 0")
-      case True
-      then show ?thesis using ac_incomparable by auto
-    next
-      case False
-      show ?thesis
+      case False show ?thesis
       proof (rule ccontr)
-        assume "\<not> (\<forall>z. a + x \<noteq> c + z)"
+        assume "\<not>(\<forall>z. a + x \<noteq> c + z)"
         then obtain z where hz: "a + x = c + z" by auto
-        then have "z \<noteq> 0" using add_zero_eq_self ac_incomparable by auto
+        with ac_incomparable have "z \<noteq> 0" by auto
         from \<open>x \<noteq> 0\<close> obtain v where "v \<in> x" by auto
-        then have "a + v \<in> c + z" unfolding hz[symmetric] using add_eq_bin_union_repl_add[of a x] by auto
+        then have "a + v \<in> c + z" using hz add_eq_bin_union_repl_add[where ?Y=x] by auto
         then consider (c) "a + v \<in> c" | (\<lambda>) "a + v \<in> lift c z" unfolding add_eq_bin_union_lift by auto
         then show "False"
-        proof (cases)
-          case c                             
+        proof cases
+          case c
           have "lift c z \<subseteq> lift a x"
           proof (rule ccontr)
-            assume "\<not> lift c z \<subseteq> lift a x"
+            assume "\<not>(lift c z \<subseteq> lift a x)"
             then have "\<exists>z' : lift c z.  z' \<in> a" using hz unfolding add_eq_bin_union_lift by auto
             then obtain w where "c + w \<in> a" using lift_eq_repl_add by auto
             then have "c + w \<in> a + v" using add_eq_bin_union_lift by auto
-            moreover have "a + v \<in> c + w" using add_eq_bin_union_lift[of c w] using c by auto
+            moreover from c have "a + v \<in> c + w" using add_eq_bin_union_lift[where ?Y=w] by auto
             ultimately show "False" using not_mem_if_mem by auto
           qed
           moreover from mem have "lift a x \<inter> lift c z = 0" for z using lift_eq_repl_add by auto
@@ -85,9 +84,15 @@ proof (rule ccontr)
           then show "False" using lift_eq_repl_add mem.IH \<open>v \<in> x\<close> by auto
         qed
       qed
-    qed
+    qed (use ac_incomparable in auto)
   qed
-  then show "False" using assms by auto
+  with assms show "False" by auto
 qed
+
+lemma additively_divides_if_add_eq_addE:
+  assumes "a + b = c + d"
+  obtains (left_divides) "a \<unlhd> c" | (right_divides) "c \<unlhd> a"
+  using assms additively_divides_or_additively_divides_if_add_eq_add by blast
+
 
 end
