HOTG/Orders/HOTG_Orders.thy
@@ -3,7 +3,7 @@ theory HOTG_Orders
   imports
     HOTG_Less_Than
     HOTG_Well_Orders
-    HOTG_Additive_Order
+    HOTG_Additively_Divides
 begin
 
 
