HOTG/Ordinals/HOTG_Ordinals.thy
@@ -3,7 +3,7 @@
 theory HOTG_Ordinals
   imports
     HOTG_Ordinals_Base
-    HOTG_Ordinals_Min_Max
+    HOTG_Ordinals_Max
     HOTG_Ranks
 begin
 
